ROOT
@@ -11,7 +11,9 @@ session "Goblint_Formalization" in "src" = "HOL-IMP" +
     "Solver"
     "Pipeline"
     "Examples"
+    "attempt2"
   theories
     Goblint_Formalization
     Scratch
     Example_Sign_Analysis
+    Attempt2_Step0
